introduce tlist and finish cont_context

theories/typing/cont_context.v
@@ -5,115 +5,78 @@ From lrust.typing Require Export lft_contexts type type_context.
 
 Set Default Proof Using "Type".
 
-Section cont_context_def.
-  Context `{!typeG Σ}.
+Notation valpl := (plist (const val)).
 
-  Definition cont_postcondition : iProp Σ := True%I.
-
-  Record cctx_elt : Type :=
-    CCtx_iscont { cctxe_k : val; cctxe_L : llctx; cctxe_As : Types; (* temp hack*)
-                  cctxe_n : nat; cctxe_T : vec val cctxe_n → tctx cctxe_As }.
-End cont_context_def.
-Add Printing Constructor cctx_elt.
-
-Notation cctx := (list cctx_elt).
-
-Notation "k ◁cont( L , T )" := (CCtx_iscont k L _ _ T)
-  (at level 70, format "k  ◁cont( L ,  T )").
+Fixpoint valpl_to_exprs {As} (vl: valpl As) : list expr :=
+  match As, vl with ^[], _ => [] |
+    _ ^:: _, v -:: vl' => (v: expr) :: valpl_to_exprs vl' end.
 
 Section cont_context.
   Context `{!typeG Σ}.
 
-  Definition cctx_elt_interp (tid : thread_id) (x : cctx_elt) : iProp Σ :=
-    let '(k ◁cont(L, T)) := x in
-    (∀ args V, na_own tid ⊤ -∗ llctx_interp L 1 -∗ tctx_interp tid (T args) V -∗
-         WP k (of_val <$> (args : list _)) {{ _, cont_postcondition }})%I.
-  Definition cctx_interp (tid : thread_id) (C : cctx) : iProp Σ :=
-    (∀ (x : cctx_elt), ⌜x ∈ C⌝ -∗ cctx_elt_interp tid x)%I.
+  Definition cont_postcondition: iProp Σ := True%I.
 
-  (* Global Instance cctx_interp_permut tid:
-    Proper ((≡ₚ) ==> (⊣⊢)) (cctx_interp tid).
-  Proof. solve_proper. Qed.
+  Record cctx_elt := CCtxe {
+    cctxe_k: val;  cctxe_L: llctx;  cctxe_As: Types;
+    cctxe_T: valpl cctxe_As → tctx cctxe_As;  cctxe_pre: predl cctxe_As;
+  }.
 
-  Lemma cctx_interp_cons tid x T :
-    cctx_interp tid (x :: T) ≡ (cctx_elt_interp tid x ∧ cctx_interp tid T)%I.
-  Proof.
-    iSplit.
-    - iIntros "H". iSplit; [|iIntros (??)]; iApply "H"; rewrite elem_of_cons; auto.
-    - iIntros "H". iIntros (? Hin). revert Hin. rewrite elem_of_cons. intros [-> |?].
-      + by iDestruct "H" as "[H _]".
-      + iDestruct "H" as "[_ H]". by iApply "H".
-  Qed.
+  Definition cctx_elt_interp (tid: thread_id) (c: cctx_elt) : iProp Σ :=
+    □ let '(CCtxe k L _ T pre) := c in ∀vl vπl,
+      na_own tid ⊤ -∗ llctx_interp L 1 -∗ tctx_interp tid (T vl) vπl -∗
+        ⟨π, pre (vπl -$ π)⟩ -∗ WP k (valpl_to_exprs vl) {{ _, cont_postcondition }}.
 
-  Lemma cctx_interp_nil tid : cctx_interp tid [] ≡ True%I.
-  Proof. iSplit; first by auto. iIntros "_". iIntros (? Hin). inversion Hin. Qed.
+End cont_context.
+Add Printing Constructor cctx_elt.
 
-  Lemma cctx_interp_app tid T1 T2 :
-    cctx_interp tid (T1 ++ T2) ≡ (cctx_interp tid T1 ∧ cctx_interp tid T2)%I.
-  Proof.
-    induction T1 as [|?? IH]; first by rewrite /= cctx_interp_nil left_id.
-    by rewrite /= !cctx_interp_cons IH assoc.
-  Qed.
+Notation cctx := (tlist cctx_elt).
 
-  Lemma cctx_interp_singleton tid x :
-    cctx_interp tid [x] ≡ cctx_elt_interp tid x.
-  Proof. rewrite cctx_interp_cons cctx_interp_nil right_id //. Qed. *)
+Notation "k ◁cont{ L , T } pre" := (CCtxe k L _ T pre)
+  (at level 55, format "k  ◁cont{ L ,  T }  pre").
 
-  (* Lemma fupd_cctx_interp tid C :
-    (|={⊤}=> cctx_interp tid C) -∗ cctx_interp tid C.
-  Proof.
-    rewrite /cctx_interp. iIntros "H". iIntros ([k L n As T]) "%".
-    iIntros (args) "HL HT". iMod "H".
-    by iApply ("H" $! (k ◁cont(L, T)) with "[%] HL HT").
-  Qed. *)
+Notation cctx_interp tid := (big_sepTL (cctx_elt_interp tid)).
 
-  (* Definition cctx_incl (E : elctx) (C1 C2 : cctx): Prop :=
-    ∀ tid, lft_ctx -∗ elctx_interp E -∗ cctx_interp tid C1 -∗ cctx_interp tid C2.
+Section cont_context.
+  Context `{!typeG Σ}.
+
+  Lemma cctx_interp_forall tid C :
+    cctx_interp tid C ⊣⊢ ∀ c, ⌜c ∈ C⌝ → cctx_elt_interp tid c.
+  Proof. by rewrite big_sepTL_forall. Qed.
+
+  Global Instance cctx_interp_permut tid :
+    Proper ((≡ₜₑ) ==> (⊣⊢)) (cctx_interp tid).
+  Proof. move=> *. rewrite !big_sepTL_forall. by do 4 f_equiv. Qed.
+
+  Definition cctx_incl (E: elctx) (C C': cctx) : Prop :=
+    ∀tid, lft_ctx -∗ proph_ctx -∗ uniq_ctx -∗
+      elctx_interp E -∗ cctx_interp tid C -∗ cctx_interp tid C'.
 
   Global Instance cctx_incl_preorder E : PreOrder (cctx_incl E).
   Proof.
-    split.
-    - iIntros (??) "_ _ $".
-    - iIntros (??? H1 H2 ?) "#LFT #HE HC".
-      iApply (H2 with "LFT HE"). by iApply (H1 with "LFT HE").
+    split; [iIntros (??) "_ _ _ _ $"|].
+    iIntros (??? In In' ?) "#LFT #PROPH #UNIQ #E ?".
+    iApply (In' with "LFT PROPH UNIQ E"). by iApply (In with "LFT PROPH UNIQ E").
   Qed.
 
   Lemma incl_cctx_incl E C1 C2 : C1 ⊆ C2 → cctx_incl E C2 C1.
   Proof.
-    rewrite /cctx_incl /cctx_interp. iIntros (HC1C2 tid) "_ #HE H * %".
-    iApply ("H" with "[%]"). by apply HC1C2.
-  Qed. *)
-(*
-  Lemma cctx_incl_cons {As} E k L n (T1 T2 : vec val n → tctx As) C1 C2 :
-    cctx_incl E C1 C2 → (∀ args, tctx_incl E L (T2 args) (T1 args)) →
-    cctx_incl E (k ◁cont(L, T1) :: C1) (k ◁cont(L, T2) :: C2).
-  Proof.
-    iIntros (HC1C2 HT1T2 ?) "#LFT #HE H". rewrite /cctx_interp.
-    iIntros (x) "Hin". iDestruct "Hin" as %[->|Hin]%elem_of_cons.
-    - iIntros (args) "Htl HL HT".
-      iMod (HT1T2 with "LFT HE HL HT") as "(HL & HT)".
-      iApply ("H" $! (_ ◁cont(_, _)) with "[%] Htl HL HT").
-      constructor.
-    - iApply (HC1C2 with "LFT HE [H] [%]"); last done.
-      iIntros (x') "%". iApply ("H" with "[%]"). by apply elem_of_cons; auto.
+    iIntros (Sub ?) "_ _ _ _ C". rewrite !cctx_interp_forall.
+    iIntros (? In). move/Sub in In. by iApply "C".
   Qed.
 
-  Lemma cctx_incl_nil E C : cctx_incl E C [].
-  Proof. apply incl_cctx_incl. by set_unfold. Qed.
+  Lemma cctx_incl_nil E C : cctx_incl E C ^[].
+  Proof. by iIntros. Qed.
 
-  (* Extra strong cctx inclusion rule that we do not have on paper. *)
-  Lemma cctx_incl_cons_dup E k L n (T1 T2 : vec val n → tctx) C1 C2 :
-    k ◁cont(L, T1) ∈ C1 →
-    (∀ args, tctx_incl E L (T2 args) (T1 args)) →
-    cctx_incl E C1 C2 →
-    cctx_incl E C1 (k ◁cont(L, T2) :: C2).
+  Lemma cctx_incl_cons {As} E k L (T T': valpl As → tctx As) tr C C' pre :
+    cctx_incl E C C' → (∀vl, tctx_incl E L (T' vl) (T vl) tr) →
+    cctx_incl E (k ◁cont{L, T} pre ^:: C) (k ◁cont{L, T'} (tr pre) ^:: C').
   Proof.
-    intros Hin ??. rewrite <-cctx_incl_cons; try done.
-    clear -Hin. iIntros (?) "_ #HE HC".
-    rewrite cctx_interp_cons. iSplit; last done. clear -Hin.
-    iInduction Hin as [] "IH"; rewrite cctx_interp_cons;
-      [iDestruct "HC" as "[$ _]" | iApply "IH"; iDestruct "HC" as "[_ $]"].
-  Qed. *)
+    iIntros (InC InT ?) "#LFT #PROPH #UNIQ #E /=#[c C]".
+    iSplit; [|by iApply InC]. iIntros "!>" (??) "Na L T' Obs".
+    iMod (InT with "LFT PROPH UNIQ E L T' Obs") as (?) "(L & Obs & T)".
+    iApply ("c" with "Na L T Obs").
+  Qed.
+
 End cont_context.
 
-(* Global Hint Resolve cctx_incl_nil cctx_incl_cons : lrust_typing. *)
+Global Hint Resolve cctx_incl_nil cctx_incl_cons : lrust_typing.
