theories/typing/bool.v
@@ -30,12 +30,13 @@ Section bool.
     typed_body E L C T (let: x := #b in e) (λ al, tr (b -:: al)).
   Proof. iIntros. iApply type_let; by [apply type_bool_instr|solve_typing]. Qed.
 
-  Lemma type_if {As} E L C (T : tctx As) e1 e2 p pre1 pre2:
-    typed_body E L C T e1 pre1 -∗ typed_body E L C T e2 pre2 -∗
-    typed_body E L C (p ◁ bool_ty +:: T) (if: p then e1 else e2)
-      (λ '(b -:: vl), if b then pre1 vl else pre2 vl).
+  Lemma type_if {As Bs} p (T: _ As) (T': _ Bs) e1 e2 pre1 pre2 tr E L C :
+    tctx_extract_ctx E L +[p ◁ bool_ty] T T' tr →
+    typed_body E L C T' e1 pre1 -∗ typed_body E L C T' e2 pre2 -∗
+    typed_body E L C T (if: p then e1 else e2)
+      (tr (λ '(b -:: vl), if b then pre1 vl else pre2 vl)).
   Proof.
-    iIntros "e1 e2". iIntros (?[??]).
+    iIntros (?) "e1 e2". iApply typed_body_tctx_incl; [done|]. iIntros (?[??]).
     iIntros "#LFT #TIME #PROPH #UNIQ #E Na L C [p T] Obs". wp_bind p.
     iApply (wp_hasty with "p"). iIntros (?? _) "_".
     iDestruct 1 as ([|]->) "%Eq"; move: Eq=> [=->]; wp_case.
